code/src/internal/result.lean
@@ -7,17 +7,17 @@ variable [GuardModule]
 open GuardModule
 
 @[simp]
-lemma Result.is_match_tt_neq_no_match (r: Result): r.is_match = tt ↔ r ≠ Result.no_match :=
+lemma Result.is_match_tt_neq_no_match { α: Type } (r: Result α): r.is_match = tt ↔ r ≠ Result.no_match :=
 by cases r; simp [Result.is_match]
 
 @[simp]
-lemma Result.is_match_ff_neq_no_match (r: Result): r.is_match = ff ↔ r = Result.no_match :=
+lemma Result.is_match_ff_neq_no_match { α: Type } (r: Result α): r.is_match = ff ↔ r = Result.no_match :=
 by cases r; simp [Result.is_match]
 
 @[simp]
-lemma Result.is_match_neq_no_match (r: Result): r.is_match ↔ r ≠ Result.no_match :=
+lemma Result.is_match_neq_no_match { α: Type } (r: Result α): r.is_match ↔ r ≠ Result.no_match :=
 by cases r; simp [Result.is_match]
 
 @[simp]
-lemma Result.not_is_match_eq_no_match (r: Result): !r.is_match ↔ r = Result.no_match :=
+lemma Result.not_is_match_eq_no_match { α: Type } (r: Result α): !r.is_match ↔ r = Result.no_match :=
 by cases r; simp [Result.is_match]
